Progress on Key Schedule

src/tls/KeySchedule.fst
@@ -27,14 +27,58 @@ open HSCrypto
 
 
 // LONG TERM GLOBAL SECRETS
+// ******************************************
 
-abstract type master_secret = b:bytes{}
-abstract type resumption_secret = b:bytes{}
+// For now, we stick to the style of miTLS 0.9
+// to avoid a circular dependency between KEF and StatefulLHAE
+
+// PRF (type pms) -> TLSInfo (type id) -> KEF (extract pms)
+//                     \ StatefulLHAE (coerce id) / 
+
+// Morally, we would like the following types to be
+// abstract, but they must be concrete in order for the definition
+// of id to appear in StatefulLHAE.
+
+// abstract type master_secret = b:bytes{}
+type pms = TLSInfo.pms
+
+// (in TLSInfo.fst)
+// type pms =
+// | DH_PMS of CommonDH.dhpms // concrete
+// | RSA_PMS of RSAKey.rsapms // concrete
+
+// Index type for keys; it is morally abstract in
+// StatefulLHAE (but has functions safeId: id->bool,
+// algId: id -> aeAlg) and its concrete definition may
+// be used to prove that StatefulLHAE.gen is not called
+// twice with the same id
+type id = TLSInfo.id
+
+// (in TLSInfo.fst)
+// type id = {
+//  msId   : msId;            // the index of the master secret used for key derivation
+//  kdfAlg : kdfAlg_t;          // the KDF algorithm used for key derivation
+//  pv     : protocolVersion; // should be part of aeAlg
+//  aeAlg  : aeAlg;           // the authenticated-encryption algorithms
+//  csrConn: csRands;         // the client-server random of the connection
+//  ext: negotiatedExtensions;// the extensions negotiated for the current session
+//  writer : role             // the role of the writer
+//  }
+
+// abstract type resumption_secret = b:bytes{}
+type resumption_secret = b:bytes{}
+
 type exporter_secret = b:bytes{}
-abstract type pre_share_key = b:bytes{}
 
-val cert_keys: ref RSAKey.RSA_PK; // 
-val ticket_key: ref bytes // TODO
+// abstract type pre_share_key = b:bytes{}
+type pre_shared_key = PSK.psk
+
+// ******************************************
+// ADL: I don't think these can be module-wide variables
+// let's encapsulate in state
+//val cert_keys: ref RSAKey.RSA_PK; 
+//val ticket_key: ref bytes // TODO
+// ******************************************
 
 type client_schedule_state =
 | C_KXS_INIT //initial state, state to get back to for renegotiation
@@ -57,32 +101,134 @@ type server_schedule_state =
 | S_KXS12_RSA
 
 type schedule_state =
-| KXS_client of client_schedule_state
-| KXS_server of server_schedule_state
+| KXS_Client of client_schedule_state
+| KXS_Server of server_schedule_state
 
-type kx_state = {
+let keyschedule
+  #r:rid{region <> root}
+  #peer:rid{peer <> root /\ HyperHeap.disjoint r peer}
+ = {
+ config: config;
  role: role;
- pv: pv;
- g: dh_group;
- dh_secret: dh_priv;
- dh_peer: dh_public;
- dh_agreed: bytes;
- kx_state: schedule_state;
+ key_index: rref r (option id);
+ pv: rref r (option pv);
+ g: rref r (option dh_group);
+ dh_secret: rref r (option dh_priv);
+ dh_share: rref r (option dh_public);
+ dh_peer: rref r (option dh_public);
+ dh_agreed: rref r (option dhpms);
+ state: rref r schedule_state;
 }
 
 //| KX_server of (pv:pv) * (g:dh_group) * (y:dh_priv) * (gy:dh_public) * (st:schedule_state)
 //| KX_client of (pv:pv) * (g:dh_group) * (x:dh_priv) * (gx:dh_pubic) * (st:schedule_state)
 
-val internal_state: Map.t rid (ref kx_state)
-let state_map = ref (const kx_state)
+// Agility parameters
+type ks_alpha = pv:protocolVersion * cs:cipherSuite * ems:bool
 
+type kx_state =
+| KS_C_Init //initial state, possibly unused, corresponds to C_Idle
+| KS_C_12_SH_Resume of cr:random * si:sessionInfo * ms:PRF.masterSecret
+| KS_C_12_SH_Full of cr:random
+| KS_C_12_Finished_Full_RSA_EMS of cr:random * sr:random * rsapms:RSAKey.key * id:PMS.dhpms
+| KS_C_12_Finished_Full_DH_EMS of cr:random * sr:random * id:PMS.dhpms * dhpms:CommonDH.secret
+| KS_C_12_Finished_Full_noEMS of cr:random * sr:random * id:TLSInfo.msId * ms:KEF.masterSecret
+| KS_C_12_Finished_Resume of cr:random * sr:random * si:sessionInfo * ms:PRF.masterSecret
+| KS_S_Init
+
+// Question: how to do partnering?
+type ks =
+| KS: #region:rid -> cfg:config -> state:rref region ks_state -> ks
+
+let create #region:rid cfg:config r:role -> ST ks
+  (requires r<>root) =
+  ST.recall_region region;
+  let ks_region = new_region region in 
+  let istate = match r with | Client -> KS_C_Init | Server -> KS_S_Init in
+  KS region cfg (ralloc ks_region istate)
+
+let ks_client_init_12 ks:ks resuming:option (sessionInfo * PRF.masterSecret)
+  -> ST (random)
+  (requires fun h0 -> sel h0 (KX.state ks) = KS_C_Init)
+  (ensures fun h0 r h1 -> True)
+  =
+  let cr = Nonces.mkHelloRandom () in
+  let ns = match resuming with
+    | None -> KS_C_12_SH_Full cr
+    | Some si,ms -> KS_C_12_SH_Resume cr si ms in
+  (KS.state ks) ns;
+  cr
+
+let ks_client_12_sh_resume ks:ks sr:random pv:protocolVersion cs:cipherSuite sid:sessionID log:bytes
+  -> ST cVerifyData
+  (requires fun h0 ->
+    let kss = sel h0 (KX.state ks) in
+    is_KS_C_12_SH_Resume kss /\
+    (let si, _ = KS_C_12_SH_Resume.si kss in
+      pv = si.protocol_version /\
+      equalBytes sid si.sessionID /\
+      cs = si.cipher_suite
+    ))
+  (ensures fun h0 r h1 -> True)
+  =
+  let KS region cfg st = ks in
+  let KS_C_12_SH_Resume cr si ms = kss in
+  let cvd = TLSPRF.verifyData (pv,cs) ms Client log in
+  st := KS_C_12_Finished_Resume cr sr si ms;
+  cvd
+
+let ks_client_12_sh_full_dh: ks:ks sr:random alpha:ks_alpha peer_share:CommonDH.share 
+  -> ST (our_share:CommonDH.share{CommonDH.group_of our_share = CommonDH.group_of peer_share})
+  (requires fun h0 ->
+    let st = sel h0 (KX.state ks) in
+    is_KS_C_12_SH_Full st \/ is_KS_C_12_SH_Resume st)
+  =
+  let (pv, cs, ems) = alpha in
+  let our_share, dhpms = dh_reponder peer_share in
+  let dhpmsId = (our_share, peer_share) in
+  let ns = 
+    if ems then KS_C_12_Finished_Full_RSA_EMS cr sr dhpms dhpmsId
+    else
+      let csr = cr @| sr in
+      let ms = TLSPRF.extract (kefAlg alpha) dhpms csr 48 in
+      let msId = StandardMS (PMS.DHPMS dhpmsid) csr (kefAlg alpha) in
+      KS_C_12_Finished_Full_Full_noEMS cr sr msId ms in
+  let KS region cfg st = ks in
+  st := ns; out_share
+
+let ks_client_12_sh_full_rsa:
+  (requires fun h0 ->
+    let st = sel h0 (KX.state ks) in
+    is_KS_C_12_SH_Full st \/ is_KS_C_12_SH_Resume st)
+
+let ks_client_12_finished_full_rsa_ems
+
+let ks_client_12_finished_full_dh_ems
+
+let ks_client_12_finished_full_noems
+
+let 
+
+(*
+  {
+    config = cfg;
+    role = r;
+    pv = None;
+    g = None;
+    dh_secret = None;
+    dh_share = None;
+    dh_peer = None;
+    dh_agreed = None;
+    state = match r with | Client -> KXS_Client C_KXS_INIT | Server -> KXS_Server S_KXS_INIT;
+  }
+*)
 
 
 // ADL: PROBLEM WITH RESUMPTION
 // Currently if handshake has set a resumption identifier and server rejects resumption it will fail for no good reason
 
 // We cannot commit to the pv and protocol mode yet
-let kx_init_client #region:rid cfg:config -> ST unit (requires fun h-> True) (ensures contains (!state_map) rid) =
+let kx_init_client #region:rid # cfg:config -> ST unit (requires fun h-> True) (ensures contains (!state_map) rid) =
     // if contains (!state_map) rid then state is C_KXS_INIT
     // create fresh sessionInfo
     // if cfg.resumption enabled
